

## Assignment 2 Double-Pipe Heat Exchanger - special case Analysis

To compute:-  $\Delta T_{LMTD}$  for a counter-flow heat exchanger

soln:-  $\Delta T_{LMTD} \rightarrow$  Log mean temperature difference

given:-  $\dot{C}_c = \dot{C}_h$  (equal heat-capacity rates)

$\rightarrow$  The ~~rate~~ rate of heat lost by the hot fluid must equal the rate of heat gained by the cold fluid:

$$\dot{Q} = \dot{C}_h (T_h^{in} - T_h^{out}) = \dot{C}_c (T_c^{out} - T_c^{in})$$

Since,  $\dot{C}_h = \dot{C}_c \Rightarrow T_h^{in} - T_h^{out} = T_c^{out} - T_c^{in}$

$$\Rightarrow T_h^{in} - T_c^{out} = T_h^{out} - T_c^{in} \quad \text{--- (1)}$$

now, For a counter-flow heat exchanger, the temperature difference at the two ends are defined as:

$$\Delta T_I = T_h^{in} - T_c^{out}$$

$$\Delta T_{II} = T_h^{out} - T_c^{in}$$

$\Rightarrow$  from (1)  $\rightarrow \Delta T_I = \Delta T_{II}$  (The temperature difference ~~at the two ends are defined~~ between the hot and cold streams is constant along the entire length of the heat exchanger)

$$\text{Let, } \Delta T_0 = \Delta T_I = \Delta T_{II}$$

$$\Rightarrow \Delta T_{LMTD} = \frac{\Delta T_I - \Delta T_{II}}{\ln\left(\frac{\Delta T_I}{\Delta T_{II}}\right)}$$

$$\rightarrow \text{putting } \Delta T_I = \Delta T_{II} = \Delta T_0$$

$$\Delta T_{LMTD} = \frac{\Delta T_0 - \Delta T_2}{\ln\left(\frac{\Delta T_0}{\Delta T_2}\right)} = \frac{0}{\ln(1)} = \frac{0}{0} \text{ (indeterminate form)}$$

$$\Rightarrow \text{Let, } \gamma = \frac{\Delta T_I}{\Delta T_{II}}$$

$$\text{now, } \lim_{\Delta T_I \rightarrow \Delta T_{II}} \Delta T_{LMTD} = \lim_{\gamma \rightarrow 1} \left[ \Delta T_{II} \cdot \frac{\gamma - 1}{\ln \gamma} \right]$$

$$\rightarrow \text{L'Hopital rule, } \lim_{\gamma \rightarrow 1} \Delta T_{II} \frac{\frac{d}{d\gamma}(\gamma - 1)}{\frac{d}{d\gamma} \ln \gamma} = \lim_{\gamma \rightarrow 1} \Delta T_{II} \frac{1}{1/\gamma} = \lim_{\gamma \rightarrow 1} \Delta T_{II} \gamma = \Delta T_{II}$$

$$\therefore \text{The limit, } \lim_{\dot{C}_c \rightarrow \dot{C}_h} \Delta T_{LMTD} = \Delta T_{II} \cdot (1) = \Delta T_0$$

$$\therefore \boxed{\lim_{\dot{C}_c \rightarrow \dot{C}_h} \Delta T_{LMTD} = \Delta T_0 = T_h^{in} - T_c^{out} = T_h^{out} - T_c^{in}}$$

$\rightarrow$  We know that for a counter-flow heat exchanger:

$$\frac{\Delta(T_h - T_c)}{T_h - T_c} = -UA \left( \frac{1}{\dot{C}_c} - \frac{1}{\dot{C}_h} \right) \text{ where } A = 2\pi r \Delta x$$

$\Rightarrow$  in differential form

$$\frac{d(\Delta T)}{dx} = -UA' \left( \frac{1}{\dot{C}_c} - \frac{1}{\dot{C}_h} \right) \Delta T$$

$\rightarrow$  applying the condition  $\dot{C}_c = \dot{C}_h$  we get,

$$\frac{d(\Delta T)}{dx} = -UA'(0) \Delta T \Rightarrow \boxed{\frac{d(\Delta T)}{dx} = 0}$$

$\rightarrow$  The exponential behavior fails because the term that governs the exponential change becomes zero for this special counter-flow case, leading to linear temperature profile instead of an exponential one.